impl/src/verifier/fstar_files/NSMain__main_simple_main.fst
@@ -1,0 +1,45 @@
+module NSMain__main_simple_main
+
+open Sequence
+open List
+open BosqueTypes
+open BosqueTerms
+open BosqueCollections
+open Util
+
+(* Type names *)
+let bTypedStringType_BAnyType = (BTypedStringType BAnyType)
+
+(* Constant Declarations *)
+let nSMain__Baz__local_const =                         
+  let ___ir_ret__ = (BInt 1) in
+  ___ir_ret__
+
+(* Default Declarations *)
+let nSMain__Baz_zexample_default =                         
+  let ___ir_ret__ = (BInt 567) in
+  ___ir_ret__
+
+(* Function Declarations *)
+val nSMain__main : (x:bosqueTerm{subtypeOf BIntType (getType x)})
+let nSMain__main  = 
+  let __tmp_4 = nSMain__Baz_zexample_default in
+  let __tmp_0_arg_3 = __tmp_4 in
+  let __tmp_0_arg_2 = (BBool true) in
+  let __tmp_0_arg_1 = (BInt 34) in
+  let __tmp_0_arg_0 = (BInt 12) in
+  let _ = assert_norm(subtypeOf BIntType (getType __tmp_0_arg_3)) in
+  let _ = assert_norm(subtypeOf BBoolType (getType __tmp_0_arg_2)) in
+  let _ = assert_norm(subtypeOf BIntType (getType __tmp_0_arg_1)) in
+  let _ = assert_norm(subtypeOf BIntType (getType __tmp_0_arg_0)) in
+  let __tmp_0 = (BnSMain__Baz __tmp_0_arg_0 __tmp_0_arg_1 __tmp_0_arg_2 __tmp_0_arg_3) in
+  let e = __tmp_0 in
+  let __tmp_6 = nSMain__Baz__local_const in
+  let _ = assert_norm(subtypeOf BIntType (getType (BInt 1))) in
+  let _ = assert_norm(subtypeOf BIntType (getType __tmp_6)) in
+  let __tmp_5 = (op_add __tmp_6 (BInt 1)) in
+  let access_example = __tmp_5 in
+  let ___ir_ret__ = access_example in
+  let __return = ___ir_ret__ in
+  __return
+
